WIP: sim init

imp/Imp2CsharpminorSepComp.v
@@ -27,6 +27,204 @@ Section PROOFALL.
 
   Import Maps.PTree.
 
+  Context `{Σ: GRA.t}.
+
+  Definition get_sge (src : Imp.programL) := Sk.load_skenv (Sk.sort (ImpMod.get_modL src).(ModL.sk)).
+  Definition get_tge (tgt : Csharpminor.program) := Genv.globalenv tgt.
+
+  Definition dummy_blk : positive := 1%positive.
+
+  Definition map_blk : programL -> nat -> Values.block :=
+    fun src blk =>
+      match (compile src) with
+      | OK tgt =>
+        if (ge_dec blk (src_init_nb src)) then Pos.of_succ_nat (2 + (ext_len src) + blk)
+        else
+          let sg := get_sge src in
+          let tg := get_tge tgt in
+          match sg.(SkEnv.blk2id) blk with
+          | Some name =>
+            match Genv.find_symbol tg (s2p name) with
+            | Some tblk => tblk
+            | None => dummy_blk
+            end
+          | None => dummy_blk
+          end
+      | _ => dummy_blk
+      end
+  .
+
+  Lemma map_blk_after_init :
+    forall src blk
+      (COMP : exists tgt, Imp2Csharpminor.compile src = OK tgt)
+      (ALLOCED : blk >= (src_init_nb src)),
+      (<<ALLOCMAP: (map_blk src blk) = Pos.of_succ_nat (2 + (ext_len src) + blk)>>).
+  Proof.
+    i. unfold map_blk. des. des_ifs.
+  Qed.
+
+  Lemma gmap_preserves_length :
+    forall src gm
+      (GAMP: get_gmap src = Some gm),
+      (<<EVL: List.length gm.(_ext_vars) = List.length src.(ext_varsL)>>) /\
+      (<<EFL: List.length gm.(_ext_funs) = List.length src.(ext_funsL)>>) /\
+      (<<IVL: List.length gm.(_int_vars) = List.length src.(prog_varsL)>>) /\
+      (<<IFL: List.length gm.(_int_funs) = List.length src.(prog_funsL)>>).
+  Proof.
+    unfold get_gmap. i. uo; des_ifs; ss. repeat split.
+    - unfold compile_eVars. eapply map_length.
+    - unfold compile_eFuns. eapply map_length.
+    - unfold compile_iVars. eapply map_length.
+    - unfold pre_compile_iFuns in Heq0. des_ifs. do 2 (rewrite List.map_map). eapply map_length.
+  Qed.
+
+  Lemma Genv_advance_next_length :
+    forall (l : list (ident * globdef fundef ())) p,
+      <<LEN: Genv.advance_next l p = Pos.of_nat ((List.length l) + (Pos.to_nat p))>>.
+  Proof.
+    i. depgen p. induction l; i; ss; clarify.
+    - sym; apply Pos2Nat.id.
+    - rewrite IHl. rewrite Pos2Nat.inj_succ. rewrite <- plus_n_Sm. ss.
+  Qed.
+
+  Lemma NoDup_norepeat :
+    forall A (l : list A), <<NOREPET: Coqlib.list_norepet l>> <-> NoDup l.
+  Proof.
+    split; induction l; i; ss; eauto.
+    - econs.
+    - inv H. econs; eauto.
+    - econs.
+    - inv H. econs; eauto. eapply IHl; eauto.
+  Qed.
+
+  Lemma perm_elements_PTree_norepeat :
+    forall A (l : list (elt * A))
+      (NOREPET: Coqlib.list_norepet (List.map fst l)),
+      <<LEN: Permutation.Permutation (elements (Maps.PTree_Properties.of_list l)) l>>.
+  Proof.
+    i. eapply Permutation.NoDup_Permutation.
+    - apply NoDup_map_inv with (f:= fst). apply NoDup_norepeat. eapply elements_keys_norepet.
+    - apply NoDup_map_inv with (f:= fst). apply NoDup_norepeat. auto.
+    - i. assert (NOREPET2: Coqlib.list_norepet (List.map fst (elements (Maps.PTree_Properties.of_list l)))).
+      { eapply elements_keys_norepet. }
+      destruct x as [ID NODE]. split; i.
+      + hexploit Maps.PTree_Properties.of_list_norepet.
+        { eapply NOREPET2. }
+        { eapply H. }
+        i. rewrite Maps.PTree_Properties.of_list_elements in H0. eapply Maps.PTree_Properties.in_of_list in H0. auto.
+      + hexploit Maps.PTree_Properties.of_list_norepet.
+        { eapply NOREPET. }
+        { eapply H. }
+        i. eapply Maps.PTree_Properties.in_of_list. rewrite Maps.PTree_Properties.of_list_elements. auto.
+  Qed.
+
+  Lemma length_elements_PTree_norepet :
+    forall A (l : list (elt * A))
+      (NOREPET: Coqlib.list_norepet (List.map fst l)),
+      <<LEN: List.length (elements (Maps.PTree_Properties.of_list l)) = List.length l>>.
+  Proof.
+    i. eapply Permutation.Permutation_length. eapply perm_elements_PTree_norepeat. auto.
+  Qed.
+
+  Lemma get_iFuns_length :
+    forall g l1 l2 (GET: get_iFuns g l1 = Some l2), List.length l1 = List.length l2.
+  Proof.
+    i. unfold get_iFuns in GET. des_ifs. rewrite List.map_map. sym; eapply map_length.
+  Qed.
+
+  Lemma wfprog_defsL_length :
+    forall src tgt
+      (COMP : Imp2Csharpminor.compile src = OK tgt)
+      (WFPROG: forall x, In x ((List.map fst src.(prog_varsL)) ++ (List.map fst src.(prog_funsL)))
+                    <-> In x (List.map fst src.(defsL))),
+      <<DEFSL: List.length src.(defsL) = List.length src.(prog_varsL) + List.length src.(prog_funsL)>>.
+  Proof.
+    i. unfold compile, _compile in COMP. des_ifs. unfold compile_gdefs in Heq0. uo; des_ifs; ss.
+    do 3 rewrite <- (map_length fst). rewrite <- app_length.
+    eapply Permutation.Permutation_length. eapply perm_elements_PTree_norepeat. auto.
+    
+
+  Lemma map_blk_init_range :
+    forall src tgt id b
+      (COMP : Imp2Csharpminor.compile src = OK tgt)
+      (WFPROG: forall x, In x ((List.map fst src.(prog_varsL)) ++ (List.map fst src.(prog_funsL)))
+                    <-> In x (List.map fst src.(defsL)))
+      (TGT: Genv.find_symbol (get_tge tgt) id = Some b),
+      <<RANGE: (b < (tgt_init_nb src))%positive>>.
+  Proof.
+    i. unfold get_tge in *. unfold compile, _compile in COMP. des_ifs. unfold compile_gdefs in Heq0.
+    uo; des_ifs; ss. unfold Genv.find_symbol in TGT. apply Genv.genv_symb_range in TGT.
+    unfold Genv.globalenv in TGT. ss. rewrite Genv.genv_next_add_globals in TGT. ss.
+    unfold tgt_init_nb. unfold ext_len, int_len. hexploit gmap_preserves_length; eauto. i; des.
+    rewrite Genv_advance_next_length in TGT. rewrite length_elements_PTree_norepet in TGT; eauto.
+    
+ 
+  Admitted.
+
+
+    
+  TGT : Coqlib.Plt b
+          (Pos.of_nat
+             (Datatypes.length
+                (List.map (fun '(n, d) => (n, lift_def g n d)) (_ext_funs g) ++
+                 List.map (fun '(n, d) => (n, lift_def g n d)) (_ext_vars g) ++
+                 (s2p "malloc", Gfun (External EF_malloc))
+                 :: (s2p "free", Gfun (External EF_free)) :: l1 ++ List.map (fun '(n, d) => (n, lift_def g n d)) (_int_vars g)) +
+              Pos.to_nat 1))
+  EVL : Datatypes.length (_ext_vars g) = Datatypes.length (ext_varsL src)
+  EFL : Datatypes.length (_ext_funs g) = Datatypes.length (ext_funsL src)
+  IVL : Datatypes.length (_int_vars g) = Datatypes.length (prog_varsL src)
+  IFL : Datatypes.length (_int_funs g) = Datatypes.length (prog_funsL src)
+  ============================
+  <<
+  (b < Pos.of_succ_nat (2 + (Datatypes.length (ext_varsL src) + Datatypes.length (ext_funsL src)) + Datatypes.length (defsL src)))%positive >>
+
+    eapply Genv.find_symbol_inversion in TGT. unfold prog_defs_names in TGT. ss.
+  Lemma map_blk_neq :
+    forall src b1 b2
+      (COMP : exists tgt, Imp2Csharpminor.compile src = OK tgt)
+      (WFPROG: forall x, In x ((List.map fst src.(prog_varsL)) ++ (List.map fst src.(prog_funsL)))
+                    <-> In x (List.map fst src.(defsL)))
+      (BLK1: b1 >= (src_init_nb src))
+      (BLK2: ~ (b2 >= (src_init_nb src))),
+      map_blk src b1 <> map_blk src b2.
+  Proof.
+    i. unfold map_blk. des_ifs; ii; rename H into CONTRA.
+    - clear g n.
+    
+
+  Lemma map_blk_inj :
+    forall src b1 b2
+      (COMP : exists tgt, Imp2Csharpminor.compile src = OK tgt)
+      (WFPROG: forall x, In x ((List.map fst src.(prog_varsL)) ++ (List.map fst src.(prog_funsL)))
+                    <-> In x (List.map fst src.(defsL))),
+      <<INJ: map_blk src b1 = map_blk src b2 -> b1 = b2>>.
+  Proof.
+    i. des. unfold map_blk. rewrite! COMP. unfold get_sge, get_tge. ii. rename H into MAP.
+
+
+
+
+    des_ifs; ss; eauto.
+    - do 2 (apply Pos.succ_inj in MAP). rewrite SuccNat2Pos.inj_iff in MAP; lia.
+    - 
+
+
+
+
+
+
+
+
+
+
+
+
+
+
+
+
+
   (* Lemma list_norepet_NoDupB {K} {decK} : *)
   (*   forall l, Coqlib.list_norepet l <-> @NoDupB K decK l = true. *)
   (* Proof. *)
@@ -128,8 +326,6 @@ Section PROOFALL.
     3: apply LPt.
     auto. auto.
   Qed.
-
-  Context `{Σ: GRA.t}.
 
   Lemma _comm_link_imp_link_mod
         src1 src2 srcl tgt1 tgt2 tgtl (ctx : ModL.t)
